Midway

main.v
@@ -12,162 +12,162 @@ Definition Graph := list (prod Node (list Node)).
 
 (* TODO := add the check to avoid duplicated edge addition *)
 Fixpoint add_edge (adj : Graph) (v1 v2: Node): Graph :=
-    match adj with
-    | nil => (cons (v1, (cons v2 nil)) nil) 
-    | (cons (x,nghbrs) adj1) => 
-            if (Nat.eqb x v1) 
-            then  (cons (x, (cons v2 nghbrs)) adj1) 
-            else (cons (x, nghbrs) (add_edge adj1 v1 v2)) 
-    end.
+      match adj with
+      | nil => (cons (v1, (cons v2 nil)) nil) 
+      | (cons (x,nghbrs) adj1) => 
+                  if (Nat.eqb x v1) 
+                  then    (cons (x, (cons v2 nghbrs)) adj1) 
+                  else (cons (x, nghbrs) (add_edge adj1 v1 v2)) 
+      end.
 
 Fixpoint construct_empty_graph (n: nat) : Graph :=
-    match n with
-    | 0 => nil
-    | (S n1) => (n,nil)::(construct_empty_graph n1)
-    end.
-    
+      match n with
+      | 0 => nil
+      | (S n1) => (n,nil)::(construct_empty_graph n1)
+      end.
+      
 Example two_nodes_empty_graph:
-    construct_empty_graph 2 = [(2,nil);(1,nil)].
+      construct_empty_graph 2 = [(2,nil);(1,nil)].
 Proof.
-    simpl. auto.
+      simpl. auto.
 Qed.
 
 
 
 (* TODO --> check that we are not adding a node that's larger than n *)
 Fixpoint construct_undir_graph (n: nat) (edge_list : list Edge): Graph := 
-    match edge_list with 
-    | nil => (construct_empty_graph n)
-    | (cons (u,v) edge_list1) => add_edge (add_edge (construct_undir_graph n edge_list1) u v) v u
-    end.
+      match edge_list with 
+      | nil => (construct_empty_graph n)
+      | (cons (u,v) edge_list1) => add_edge (add_edge (construct_undir_graph n edge_list1) u v) v u
+      end.
 
 Fixpoint construct_dir_graph (n: nat) (edge_list : list Edge): Graph := 
-    match edge_list with 
-    | nil => (construct_empty_graph n)
-    | (cons (u,v) edge_list1) => add_edge (construct_dir_graph n edge_list1) u v
-    end.
+      match edge_list with 
+      | nil => (construct_empty_graph n)
+      | (cons (u,v) edge_list1) => add_edge (construct_dir_graph n edge_list1) u v
+      end.
 
 Example null_graph:=
-    construct_undir_graph 0 nil.
+      construct_undir_graph 0 nil.
 Example null_graph_is_null:
-    null_graph = nil.
+      null_graph = nil.
 Proof.
-    auto.
+      auto.
 Qed.
 
 
 Example two_cycle:=
-    construct_undir_graph 2 [(1,2)].
+      construct_undir_graph 2 [(1,2)].
 Example two_cycle_is_correct:
-    two_cycle = [(2,[1]);(1,[2])].
+      two_cycle = [(2,[1]);(1,[2])].
 Proof.
-    simpl. auto.
+      simpl. auto.
 Qed.
 
 Example one_line:=
-    construct_dir_graph 2 [(1,2)].
+      construct_dir_graph 2 [(1,2)].
 Example one_line_is_correct:
-    one_line = [(2,[]);(1,[2])].
+      one_line = [(2,[]);(1,[2])].
 Proof.
-    simpl. auto.
+      simpl. auto.
 Qed.
 
 
 
 
-(* Todo  ---> Prove that construct_graph function is correct. *)
+(* Todo ---> Prove that construct_graph function is correct. *)
 
 
-    
+      
 
 Fixpoint get_all_neighbors (g: Graph) (u : Node): (list Node):=
-    match g with
-    | nil => nil
-    | (v,e)::g1 => 
-                if (Nat.eqb u v) 
-                    then e ++ (get_all_neighbors g1 u)
-                else
-                    let n1 := (get_all_neighbors g1 u) in 
-                    if (andb (existsb (Nat.eqb u) e)  (negb (existsb (Nat.eqb v) n1)))
-                        then v::n1
-                    else n1
-    end.
+      match g with
+      | nil => nil
+      | (v,e)::g1 => 
+                        if (Nat.eqb u v) 
+                              then e ++ (get_all_neighbors g1 u)
+                        else
+                              let n1 := (get_all_neighbors g1 u) in 
+                              if (andb (existsb (Nat.eqb u) e)    (negb (existsb (Nat.eqb v) n1)))
+                                    then v::n1
+                              else n1
+      end.
 
 Fixpoint get_children (g: Graph) (u : Node): (list Node):=
-    match g with
-    | nil => nil
-    | (v,e)::g1 => 
-                if (Nat.eqb u v) 
-                    then e 
-                else
-                    get_children g1 u
-    end.
+      match g with
+      | nil => nil
+      | (v,e)::g1 => 
+                        if (Nat.eqb u v) 
+                              then e 
+                        else
+                              get_children g1 u
+      end.
 
 
 Example all_nghbrs_of_1_in_two_cycle:
-    get_all_neighbors two_cycle 1 = [2].
+      get_all_neighbors two_cycle 1 = [2].
 Proof.
-    simpl. auto.
+      simpl. auto.
 Qed.
 
 Example actual_nghbrs_of_1_in_one_line:
-    get_children one_line 1 = [2].
+      get_children one_line 1 = [2].
 Proof.
-    simpl. auto.
+      simpl. auto.
 Qed.
 
 Example actual_nghbrs_of_2_in_one_line:
-    get_children one_line 2 = nil.
+      get_children one_line 2 = nil.
 Proof.
-    simpl. auto.
+      simpl. auto.
 Qed.
 
 
 Fixpoint is_connected (g : Graph) : Prop:=
-    match g with 
-    | nil => True
-    | (v,e)::g1 => let n := get_all_neighbors g v in 
-                    match n with
-                    | nil => False
-                    | _ => is_connected g1
-                    end
-    end.
-    
-    
+      match g with 
+      | nil => True
+      | (v,e)::g1 => let n := get_all_neighbors g v in 
+                              match n with
+                              | nil => False
+                              | _ => is_connected g1
+                              end
+      end.
+      
+      
 
 
 Example null_graph_is_connected:
-    is_connected null_graph.
+      is_connected null_graph.
 Proof.
-    simpl. auto.
+      simpl. auto.
 Qed.
 
 Example one_line_is_connected:
-    is_connected one_line.
+      is_connected one_line.
 Proof.
-    simpl. auto.
+      simpl. auto.
 Qed.
 
 Example one_line_one_node:=
-    construct_dir_graph 3 [(1,2)].
+      construct_dir_graph 3 [(1,2)].
 
 Example one_line_one_node_is_not_connected:
-    not (is_connected one_line_one_node).
+      not (is_connected one_line_one_node).
 Proof.
-    simpl. auto.
+      simpl. auto.
 Qed.
 
 (* Fixpoint is_reachable_in_k_steps (u v: Node) (k: nat): Prop :=
-    match k with
-    | 0 => if (Nat.eqb u v) then True else False
-    | S => 
+      match k with
+      | 0 => if (Nat.eqb u v) then True else False
+      | S => 
 Fixpoint get_reachable_nodes_helper (g:Graph) (list_u: list Node) (list_seen : list Node): (list Node) :=
-    match list_u with 
-    | nil => nil
-    | v::l => if (existsb (Nat.eqb v) list_seen)
-                    then (get_reachable_nodes_helper g l list_seen)
-                else v::(get_reachable_nodes_helper g ((get_actual_neighbors g v) ++ l ) (v::list_seen))
-    end.
+      match list_u with 
+      | nil => nil
+      | v::l => if (existsb (Nat.eqb v) list_seen)
+                              then (get_reachable_nodes_helper g l list_seen)
+                        else v::(get_reachable_nodes_helper g ((get_actual_neighbors g v) ++ l ) (v::list_seen))
+      end.
 
 Fixpoint is_cyclic_direc (g: Graph) : Prop := *)
 
@@ -175,15 +175,15 @@ Fixpoint is_cyclic_direc (g: Graph) : Prop := *)
 
 (* Size of the Graph: Number of Nodes in the Graph *)
 Fixpoint get_size (g : Graph) : nat :=
-  match g with
-  | nil => 0
-  | (v, _) :: g' => 1 + get_size g'
-  end.
+    match g with
+    | nil => 0
+    | (v, _) :: g' => 1 + get_size g'
+    end.
 
 Definition example_graph1 := [(1, [2; 3]); (2, [1; 3]); (3, [1; 2])].
 Example example_graph1_size : get_size example_graph1 = 3.
 Proof. reflexivity. Qed.
-  
+    
 Definition example_graph2 := [(1, []); (2, [1])].
 Example example_graph2_size : get_size example_graph2 = 2.
 Proof. reflexivity. Qed.
@@ -199,52 +199,52 @@ Proof. reflexivity. Qed.
 
 (* Implementing degrees of vertices *)
 Fixpoint degree (g : Graph) (v : Node) : nat :=
-  match g with
-  | [] => 0
-  | (u, neighbors) :: rest =>
-    if Nat.eqb u v then length neighbors
-    else degree rest v
-  end.
+    match g with
+    | [] => 0
+    | (u, neighbors) :: rest =>
+      if Nat.eqb u v then length neighbors
+      else degree rest v
+    end.
 
 (* Some example *)
 Example degree_example_1 : degree [(1, [2; 3]); (2, [1; 3]); (3, [1; 2])] 1 = 2.
 Proof.
-    reflexivity.
+      reflexivity.
 Qed.
 
 Example degree_example_2 : degree [(1, [2; 3]); (2, [1; 3; 4; 5]); (3, [1; 2])] 2 = 4.
 Proof.
-    reflexivity.
+      reflexivity.
 Qed.
 
 (* Lemma: Degree of vertices of an empty graph is always 0 *)
 Lemma degree_empty_graph : forall v, degree [] v = 0.
 Proof.
-    intros v. reflexivity.
+      intros v. reflexivity.
 Qed.
 
 (* Lemma: Degree of vertices of a single vertex is always 0 *)
 Lemma degree_single_vertex : forall v u, v <> u -> degree [(u, [])] v = 0.
 Proof.
-    intros v u H. simpl. destruct (Nat.eqb_spec u v); auto.
+      intros v u H. simpl. destruct (Nat.eqb_spec u v); auto.
 Qed.
 
 (* Lemma: Degree of vertices is always positive *)
 Lemma degree_positive : forall g v,
-  0 <= degree g v.
+    0 <= degree g v.
 Proof.
-    intros.
-    induction g.
-    - simpl. lia.
-    - simpl. destruct a as[u neighbors].
-        * apply Nat.le_0_l.     
+      intros.
+      induction g.
+      - simpl. lia.
+      - simpl. destruct a as[u neighbors].
+            * apply Nat.le_0_l.     
 Qed.
 
 
 (* The degree of vertices of a graph increases when we add an edge *)
 Lemma degree_add_edge : forall g v1 v2 v,
-  In v (fst (split g)) ->
-  (v = v1 \/ v = v2) -> degree (add_edge g v1 v2) v = S (degree g v).
+    In v (fst (split g)) ->
+    (v = v1 \/ v = v2) -> degree (add_edge g v1 v2) v = S (degree g v).
 Proof.
 Admitted.
 
@@ -255,145 +255,145 @@ Admitted.
 (* //////////////////////// BFS and Diameter below //////////////////////*)
 
 (* 
-    TO Calculate the DIAMETER of the graph 
-    We just assume that the diameter will be calculated only for connected graphs. ??
-    Diameter = longest shortest path between any 2 pair of nodes
-    - need the shortest distance between all pair of nodes
-    - Then need the max value among all those
+      TO Calculate the DIAMETER of the graph 
+      We just assume that the diameter will be calculated only for connected graphs. ??
+      Diameter = longest shortest path between any 2 pair of nodes
+      - need the shortest distance between all pair of nodes
+      - Then need the max value among all those
 *)
 
 (* Random Notes for BFS 
-    do the fuel implementation: 
-    1. can just do if it returns x then x is the right answer --> so can do that 
-    fuel is at a certain equal to the number of nodes in the graph 
-    if I am showing that they are very specific element then would have to deal with the case 
-    and prove for completeness where if it returns None then what is it because the fuel runs out 
-    or just when fuel is empty why this can never be the case
+      do the fuel implementation: 
+      1. can just do if it returns x then x is the right answer --> so can do that 
+      fuel is at a certain equal to the number of nodes in the graph 
+      if I am showing that they are very specific element then would have to deal with the case 
+      and prove for completeness where if it returns None then what is it because the fuel runs out 
+      or just when fuel is empty why this can never be the case
 *)
 
 (* Fixpoint bfs_helper_measure (g : Graph) (queue : list (list Node)) (visited : list Node) (distance : nat) (target : Node) : nat :=
-  length queue.
+    length queue.
 
 Lemma bfs_helper_measure_decreasing : forall g queue visited distance target,
-  length (queue) > length (queue ++ []) ->
-  bfs_helper_measure g queue visited distance target > bfs_helper_measure g (queue ++ []) visited distance target.
+    length (queue) > length (queue ++ []) ->
+    bfs_helper_measure g queue visited distance target > bfs_helper_measure g (queue ++ []) visited distance target.
 Proof.
-  intros.
-  rewrite app_length in H.
-  simpl in H.
-  lia.
+    intros.
+    rewrite app_length in H.
+    simpl in H.
+    lia.
 Qed. *)
 
 
 (* 
-    BFS to find the shortest path from source to target
-    Returns a nat which is the shortest distance between source and target
-    or returns None if there is no path
+      BFS to find the shortest path from source to target
+      Returns a nat which is the shortest distance between source and target
+      or returns None if there is no path
 *)
 
 (* Fixpoint bfs_helper (g : Graph) (queue : list (list Node)) (visited : list Node) (distance : nat) 
 (target : Node): option nat :=
-  match queue with
-  | [] => None
-  | path :: queue' =>
-    let cur := hd 0 path in
-    if Nat.eqb cur target then Some distance
-    else if existsb (Nat.eqb cur) visited then bfs_helper g queue' visited distance target
-    else let neighbors := get_children g cur in
-         let new_paths := map (fun n => n :: path) neighbors in
-         let queue'' := (queue' ++ new_paths) in
-         bfs_helper g queue'' (cur :: visited) (S distance) target
-  end. *)
+    match queue with
+    | [] => None
+    | path :: queue' =>
+      let cur := hd 0 path in
+      if Nat.eqb cur target then Some distance
+      else if existsb (Nat.eqb cur) visited then bfs_helper g queue' visited distance target
+      else let neighbors := get_children g cur in
+             let new_paths := map (fun n => n :: path) neighbors in
+             let queue'' := (queue' ++ new_paths) in
+             bfs_helper g queue'' (cur :: visited) (S distance) target
+    end. *)
 
 (* Fixpoint bfs_helper (g : Graph) (queue : list (list Node)) (visited : list Node)
-  (distance : nat) (target : Node) (termination_counter : nat): option nat :=
-    match termination_counter with
-    | O => None
-    | S n =>
-        match queue with
-            | [] => None
-            | path :: queue' =>
-                let cur := hd 0 path in
-                (* let num_nodes_visited := length path in *)
-                if Nat.eqb cur target then Some distance
-                else if existsb (Nat.eqb cur) visited then bfs_helper g queue' visited distance target (S n)
-                else let neighbors := get_all_neighbors g cur in
-                let new_paths := map (fun n => n :: path) neighbors in
-                let queue'' := queue' ++ new_paths in
-                bfs_helper g queue'' (cur :: visited) (S distance) target n
-        end
+    (distance : nat) (target : Node) (termination_counter : nat): option nat :=
+      match termination_counter with
+      | O => None
+      | S n =>
+            match queue with
+                  | [] => None
+                  | path :: queue' =>
+                        let cur := hd 0 path in
+                        (* let num_nodes_visited := length path in *)
+                        if Nat.eqb cur target then Some distance
+                        else if existsb (Nat.eqb cur) visited then bfs_helper g queue' visited distance target (S n)
+                        else let neighbors := get_all_neighbors g cur in
+                        let new_paths := map (fun n => n :: path) neighbors in
+                        let queue'' := queue' ++ new_paths in
+                        bfs_helper g queue'' (cur :: visited) (S distance) target n
+            end
 end. *)
 
 
 (* Definition bfs_shortest_path_distance (g : Graph) (source target : Node) : option nat :=
-    bfs_helper g [[source]] [] 0 target get_size(g). *)
+      bfs_helper g [[source]] [] 0 target get_size(g). *)
 
 (* Fixpoint termination_helper (v: valuation) (c: cmd) (counter: nat) : valuation * cmd :=
 match counter with
-    | O => (v, c)
-    | S counter =>
-        match eval_cmd_once v c with
-            | Some (v', c') => eval_cmd_n v' c' fuel
-            | None => (v, c)
-        end
+      | O => (v, c)
+      | S counter =>
+            match eval_cmd_once v c with
+                  | Some (v', c') => eval_cmd_n v' c' fuel
+                  | None => (v, c)
+            end
 end. *)
 
 (* Function to get all pairs of nodes *)
 Fixpoint all_pairs (l : list Node) : list (Node * Node) :=
-  match l with
-  | nil => nil
-  | x :: xs => map (pair x) xs ++ all_pairs xs
-  end.
+    match l with
+    | nil => nil
+    | x :: xs => map (pair x) xs ++ all_pairs xs
+    end.
 
-  Example example_1: all_pairs [1; 2; 3] = [(1, 2); (1, 3); (2, 3)].
-  Proof. reflexivity. Qed.
-  
-  Example example_2: all_pairs [4; 5] = [(4, 5)].
-  Proof. reflexivity. Qed.
-  
-  Example example_3: all_pairs [6] = [].
-  Proof. reflexivity. Qed.
+    Example example_1: all_pairs [1; 2; 3] = [(1, 2); (1, 3); (2, 3)].
+    Proof. reflexivity. Qed.
+    
+    Example example_2: all_pairs [4; 5] = [(4, 5)].
+    Proof. reflexivity. Qed.
+    
+    Example example_3: all_pairs [6] = [].
+    Proof. reflexivity. Qed.
 
 
 (* Definition diameter (g : Graph) (nodes : list Node) : nat :=
-    match nodes with
-    | nil => None
-    | _ =>
-      let distances := map (fun p => bfs_shortest_path_distance g (fst p) (snd p)) (all_pairs nodes) in
-      let max_distance := fold_left (fun d opt_dist => match opt_dist with Some dist => max d dist | None => d end) distances 0 in
-      Some max_distance
-    end. *)
+      match nodes with
+      | nil => None
+      | _ =>
+          let distances := map (fun p => bfs_shortest_path_distance g (fst p) (snd p)) (all_pairs nodes) in
+          let max_distance := fold_left (fun d opt_dist => match opt_dist with Some dist => max d dist | None => d end) distances 0 in
+          Some max_distance
+      end. *)
 
 
 (* Function to calculate the diameter of a graph *)
 (* Definition diameter (g : Graph) : nat :=
-    let dist_from_source (source : Node) :=
-      let rec bfs (queue : list (Node * nat)) (visited : list Node) : nat :=
-        match queue with
-        | [] => O
-        | (cur, d) :: queue' =>
-          if existsb (Nat.eqb cur) visited then bfs queue' visited
-          else let neighbors := get_all_neighbors g cur in
-               let new_queue := queue' ++ map (fun n => (n, S d)) neighbors in
-               bfs new_queue (cur :: visited)
-        end
-      in bfs [(source, O)] []
-    in let all_nodes := map fst g in
-       let distances := map dist_from_source all_nodes in
-       fold_right max 0 distances. *)
-  
-  (* Some Examples to start with *)
-  
-  (* Example one_line :=
-    construct_undir_graph 2 [(1, 2)].
-  
-  Example null_graph :=
-    construct_undir_graph 0 nil.
+      let dist_from_source (source : Node) :=
+          let rec bfs (queue : list (Node * nat)) (visited : list Node) : nat :=
+            match queue with
+            | [] => O
+            | (cur, d) :: queue' =>
+                if existsb (Nat.eqb cur) visited then bfs queue' visited
+                else let neighbors := get_all_neighbors g cur in
+                       let new_queue := queue' ++ map (fun n => (n, S d)) neighbors in
+                       bfs new_queue (cur :: visited)
+            end
+          in bfs [(source, O)] []
+      in let all_nodes := map fst g in
+           let distances := map dist_from_source all_nodes in
+           fold_right max 0 distances. *)
+    
+    (* Some Examples to start with *)
+    
+    (* Example one_line :=
+      construct_undir_graph 2 [(1, 2)].
+    
+    Example null_graph :=
+      construct_undir_graph 0 nil.
 
-  Compute (diameter one_line). (* Output: 1 *)
-  Compute (diameter null_graph). (* Output: 0 *)
-   *)
-  (* Add some proofs for bfs and diameter *)
+    Compute (diameter one_line). (* Output: 1 *)
+    Compute (diameter null_graph). (* Output: 0 *)
+     *)
+    (* Add some proofs for bfs and diameter *)
 
 
 
@@ -405,162 +405,162 @@ Fixpoint all_pairs (l : list Node) : list (Node * Node) :=
 (*  Small Step Semantics Definition of DFS *)
 
 (* 
-    Defines 3 different kinds of steps
-    -  A node that has already been visited
-    -  A node that has not yet been visited
-    -  DFS Initialization
+      Defines 3 different kinds of steps
+      -   A node that has already been visited
+      -   A node that has not yet been visited
+      -   DFS Initialization
 *)
 Inductive DfsStep : Graph * list Node * list Node -> Graph * list Node * list Node -> Prop :=
 | DfsStepVisited : forall g vis st v,
-    ~ In v vis -> DfsStep (g, vis, v :: st) (g, v :: vis, (get_children g v) ++ st)
+      ~ In v vis -> DfsStep (g, vis, v :: st) (g, v :: vis, (get_children g v) ++ st)
 | DfsStepVisit : forall g vis st v,
-    In v vis -> DfsStep (g, vis, v :: st) (g, vis, st)
+      In v vis -> DfsStep (g, vis, v :: st) (g, vis, st)
 | DfsStepStart : forall g v,
-    DfsStep (g, [], []) (g, [], [v]).
+      DfsStep (g, [], []) (g, [], [v]).
 
 (* 
-    Defines the properties of the small step semantics
-    -  Reflexivity
-    -  Transitivity
+      Defines the properties of the small step semantics
+      -   Reflexivity
+      -   Transitivity
 *)
 Inductive DfsStepStar : Graph * list Node * list Node -> Graph * list Node * list Node -> Prop :=
 | DfsStepRefl : forall g vis st,
-    DfsStepStar (g, vis, st) (g, vis, st)
+      DfsStepStar (g, vis, st) (g, vis, st)
 | DfsStepStarOnce : forall g vis1 vis2 vis3 st1 st2 st3,
-    DfsStep (g, vis1, st1) (g, vis2, st2) -> DfsStepStar (g, vis2, st2) (g, vis3, st3) -> DfsStepStar (g, vis1, st1) (g, vis3, st3).
-    
+      DfsStep (g, vis1, st1) (g, vis2, st2) -> DfsStepStar (g, vis2, st2) (g, vis3, st3) -> DfsStepStar (g, vis1, st1) (g, vis3, st3).
+      
 (* 
-    Now let us verify that the small step semantics defined above works on some sample graphs
+      Now let us verify that the small step semantics defined above works on some sample graphs
 
-    Consider a graph with the following adjacency list. The graph has been illustrated below for further clarity.
-        1: 2, 5
-        2: 3, 7
-        3: 4
-        4: 9
-        5: 7
-        6: 8
-        7:
-        8:
-        9:
+      Consider a graph with the following adjacency list. The graph has been illustrated below for further clarity.
+            1: 2, 5
+            2: 3, 7
+            3: 4
+            4: 9
+            5: 7
+            6: 8
+            7:
+            8:
+            9:
 
-        1 --> 2 --> 3 --> 4 --> 9
-        |     |     ^              
-        v     v     |              
-        5 --> 7 ----+              
-            
-        6 --> 8
+            1 --> 2 --> 3 --> 4 --> 9
+            |     |     ^               
+            v     v     |               
+            5 --> 7 ----+               
+                  
+            6 --> 8
 *)
 
 Definition sample_graph := 
-    construct_dir_graph 9 [(1,2); (1,5); (2,3); (2,7); (3,4); (4,9); (5,7); (7,3); (6,8)].
+      construct_dir_graph 9 [(1,2); (1,5); (2,3); (2,7); (3,4); (4,9); (5,7); (7,3); (6,8)].
 
 Example dfs_step_identity:
-    DfsStep(sample_graph,[],[1])(sample_graph,[1],[2;5]).
+      DfsStep(sample_graph,[],[1])(sample_graph,[1],[2;5]).
 Proof.
-    econstructor. auto.
+      econstructor. auto.
 Qed.
 
 Example dfs_identity_step_star:
-    DfsStepStar(sample_graph,[],[1])(sample_graph,[1],[2;5]).
+      DfsStepStar(sample_graph,[],[1])(sample_graph,[1],[2;5]).
 Proof.
-    repeat econstructor. auto.
+      repeat econstructor. auto.
 Qed.
 
 Lemma dfs_step_from_one_to_four:
-    exists vis st, DfsStepStar(sample_graph, [], [1])(sample_graph, 4::vis, st).
+      exists vis st, DfsStepStar(sample_graph, [], [1])(sample_graph, 4::vis, st).
 Proof.
-    repeat econstructor. 
-    - auto.
-    - unfold not. simpl. intros. destruct H. lia. lia.
-    - unfold not. simpl. intros. destruct H. lia. lia.
-    - unfold not. simpl. intros. destruct H. lia. lia.
+      repeat econstructor. 
+      - auto.
+      - unfold not. simpl. intros. destruct H. lia. lia.
+      - unfold not. simpl. intros. destruct H. lia. lia.
+      - unfold not. simpl. intros. destruct H. lia. lia.
 Qed.
 
 Lemma dfs_step_from_five_to_nine:
-    exists vis st, DfsStepStar(sample_graph, [], [5])(sample_graph, 9::vis, st).
+      exists vis st, DfsStepStar(sample_graph, [], [5])(sample_graph, 9::vis, st).
 Proof.
-    repeat econstructor. 
-    - auto.
-    - unfold not. simpl. intros. destruct H. lia. lia.
-    - unfold not. simpl. intros. destruct H. lia. lia.
-    - unfold not. simpl. intros. destruct H. lia. lia.
-    - unfold not. simpl. intros. destruct H. lia. lia.
+      repeat econstructor. 
+      - auto.
+      - unfold not. simpl. intros. destruct H. lia. lia.
+      - unfold not. simpl. intros. destruct H. lia. lia.
+      - unfold not. simpl. intros. destruct H. lia. lia.
+      - unfold not. simpl. intros. destruct H. lia. lia.
 Qed.
 
 
 
 (* 
-    Next we define a fuel based implementation of the dfs algorithm
+      Next we define a fuel based implementation of the dfs algorithm
 *)
 
 Fixpoint dfs_helper (g : Graph) (visited stack : list Node) (fuel : nat) : list Node :=
-  match fuel with
-  | 0 => visited
-  | S fuel' =>
-      match stack with
-      | [] => visited
-      | vertex :: rem =>
-          if (existsb (Nat.eqb vertex) visited)
-            then dfs_helper g visited rem fuel'
-            else dfs_helper g ([vertex] ++ visited) ((get_children g vertex) ++ rem) fuel'
-      end
-  end.
+    match fuel with
+    | 0 => visited
+    | S fuel' =>
+          match stack with
+          | [] => visited
+          | vertex :: rem =>
+                if (existsb (Nat.eqb vertex) visited)
+                  then dfs_helper g visited rem fuel'
+                  else dfs_helper g ([vertex] ++ visited) ((get_children g vertex) ++ rem) fuel'
+          end
+    end.
 
 Definition dfs (g : Graph) (start : Node) : list Node :=
-    dfs_helper g [] [start] (length g).
+      dfs_helper g [] [start] ((length g)*(length g)).
 
 (* 
-    Again, let us verify the behaviour of the fuel based definition of DFS
-    Consider the sample graph from above.
+      Again, let us verify the behaviour of the fuel based definition of DFS
+      Consider the sample graph from above.
 
-        1 --> 2 --> 3 --> 4 --> 9
-        |     |     ^              
-        v     v     |              
-        5 --> 7 ----+              
-            
-        6 --> 8
+            1 --> 2 --> 3 --> 4 --> 9
+            |     |     ^               
+            v     v     |               
+            5 --> 7 ----+               
+                  
+            6 --> 8
 *)
 
 Lemma dfs_from_one_visits_one:
-    In 1 (dfs sample_graph 1).
+      In 1 (dfs sample_graph 1).
 Proof.
-    simpl. lia.
+      simpl. lia.
 Qed.
 
 Lemma dfs_from_one_visits_four:
-    In 4 (dfs sample_graph 1).
+      In 4 (dfs sample_graph 1).
 Proof.
-    simpl. lia.
+      simpl. lia.
 Qed.
 
 Lemma dfs_from_five_visits_nine:
-    In 5 (dfs sample_graph 1).
+      In 5 (dfs sample_graph 1).
 Proof.
-    simpl. lia.
+      simpl. lia.
 Qed.
 
 Lemma dfs_from_five_does_not_visit_nine:
-    ~ In 6 (dfs sample_graph 5).
+      ~ In 6 (dfs sample_graph 5).
 Proof.
-    simpl. unfold not. intros. 
-    destruct H. lia.
-    destruct H. lia.
-    destruct H. lia.
-    destruct H. lia.
-    destruct H. lia.
-    destruct H.
+      simpl. unfold not. intros. 
+      destruct H. lia.
+      destruct H. lia.
+      destruct H. lia.
+      destruct H. lia.
+      destruct H. lia.
+      destruct H.
 Qed.
 
 Theorem dfs_implies_dfs_step: 
-    forall g start v, In v (dfs_helper g [start] [] 1) -> exists visited stack, DfsStepStar(g, [], [start])(g, v::visited, stack).
+      forall g start v, In v (dfs_helper g [start] [] 1) -> exists visited stack, DfsStepStar(g, [], [start])(g, v::visited, stack).
 Proof.
-    intros. simpl in H. destruct H. rewrite H. repeat econstructor. auto. lia.    
+      intros. simpl in H. destruct H. rewrite H. repeat econstructor. auto. lia.      
 Qed.
 
 (* 
-    Here, we prove that our step semantics for DFS only visits a node one time.
+      Here, we prove that our step semantics for DFS only visits a node one time.
 
-    First, we define a helper lemma that helps us reason about lists.
+      First, we define a helper lemma that helps us reason about lists.
 *)
 
 Lemma not_cons_self : forall (A : Type) (x : A) (l : list A), l <> x :: l.
@@ -570,119 +570,233 @@ intro H.
 induction l as [| y l' IHl].
 - discriminate H. 
 - injection H as H1 H2. rewrite H1 in H2.
-  apply IHl in H2.
-  contradiction.
+    apply IHl in H2.
+    contradiction.
 Qed.
 
 
 (* 
-    The below theorem shows that any step dfs takes must result in only new values being added to visited.
+      The below theorem shows that any step dfs takes must result in only new values being added to visited.
 *)
 
 Theorem dfs_step_has_unique_values_in_visited:
-    forall g v visited stack stack', DfsStep(g, visited, stack)(g, v::visited, stack') -> ~ In v visited.
+      forall g v visited stack stack', DfsStep(g, visited, stack)(g, v::visited, stack') -> ~ In v visited.
 Proof.
-    intros. repeat econstructor. 
-    intro. inversion H. subst. 
-    - contradiction. 
-    - apply not_cons_self in H5. contradiction. 
+      intros. repeat econstructor. 
+      intro. inversion H. subst. 
+      - contradiction. 
+      - apply not_cons_self in H5. contradiction. 
 Qed.
 
-(* 
-    Shortest Path Between nodes A and B
-    
-    We now define a function that computes the shortest path between 2 nodes A nd B in a graph
-    
-    It does this by iteratively checking the shortest path to the destination from all of 
-    the neighbour's of the source and choosing the minimum of those paths. 
 
-    It does this recursively until it gets the shortes path if such a path exists
+(* 
+      Shortest Path Between nodes A and B
+      
+      We now define a function that computes the shortest path between 2 nodes A nd B in a graph
+      
+      It does this by iteratively checking the shortest path to the destination from all of 
+      the neighbour's of the source and choosing the minimum of those paths. 
+
+      It does this recursively until it gets the shortes path if such a path exists
 
 *)
 
-Fixpoint shortest_path_helper (g: Graph) (srcs : list Node) (dst: Node) (visited: list Node) (fuel: nat): list Node  :=
-  match fuel with
-  | 0 => []
-  | S fuel' =>
-    match srcs with
-    | [] => []
-    | src :: xsrcs => (
-        let min_rest_path := (shortest_path_helper g xsrcs dst visited fuel') in
-        let curr_path := src::(shortest_path_helper g (get_children g src) dst (src::visited) fuel') in
-        if (Nat.eqb src dst) then
-            [src]
-        else if (existsb (Nat.eqb src) visited) then
-            min_rest_path
-        else if (Nat.eqb (length min_rest_path) 0) then
-            curr_path
-        else if (Nat.leb (length min_rest_path) (length curr_path)) then
-            min_rest_path
-        else
-            curr_path
-    )
-    end
-  end.
+Fixpoint shortest_path_helper (g: Graph) (srcs : list Node) (dst: Node) (visited: list Node) (fuel: nat): list Node :=
+    match fuel with
+    | 0 => []
+    | S fuel' =>
+      match srcs with
+      | [] => []
+      | src :: xsrcs => (
+            let min_rest_path := (shortest_path_helper g xsrcs dst visited fuel') in
+            let curr_path := src::(shortest_path_helper g (get_children g src) dst (src::visited) fuel') in
+            if (Nat.eqb src dst) then
+                  [src]
+            else if (existsb (Nat.eqb src) visited) then
+                  min_rest_path
+            else if (Nat.eqb (length min_rest_path) 0) then
+                  curr_path
+            else if (Nat.leb (length min_rest_path) (length curr_path)) then
+                  min_rest_path
+            else
+                  curr_path
+      )
+      end
+    end.
 
 (* Compute shortest_path_helper another_sample_graph (get_children another_sample_graph 3) 8 [3] 99. *)
 (* Compute shortest_path_helper another_sample_graph [1] 8 [] 99. *)
 
 Definition shortest_path (g: Graph) (src: Node) (dst: Node) : list Node :=
-    let path := (shortest_path_helper g [src] dst [] ((length g)*(length g))) in
-    match rev path with 
-    | v::l => if (Nat.eqb v dst) then   
-                path
-              else  
-                []
-    | _ => []
-    end.
+      let path := (shortest_path_helper g [src] dst [] ((length g)*(length g))) in
+      match rev path with 
+      | v::l => if (Nat.eqb v dst) then    
+                        path
+                      else  
+                        []
+      | _ => []
+      end.
 
 
 (* 
-    We verify the working of the shortest path computation using the following sample graph
-    1---2---3
-    |\  |   |
-    | \ |   |
-    4   5   |
-    |   |   |
-    6---7---8
-        |   
-        9
+      We verify the working of the shortest path computation using the following sample graph
+      1---2---3
+      |\  |    |
+      | \ |    |
+      4    5    |
+      |    |    |
+      6---7---8
+            |    
+            9
 *)
 
 Definition another_sample_graph := 
-    construct_dir_graph 9 [(1,2); (1,5); (1,4); (2,3); (2,5); (3,8); (4,6); (5,7); (6,7); (7,8); (7,9)].
+      construct_dir_graph 9 [(1,2); (1,5); (1,4); (2,3); (2,5); (3,8); (4,6); (5,7); (6,7); (7,8); (7,9)].
 
 Lemma shortest_path_from_one_to_one:
-    (shortest_path another_sample_graph 1 1) = [1].
+      (shortest_path another_sample_graph 1 1) = [1].
 Proof.
-    auto.
+      auto.
 Qed.
 
 Lemma shortest_path_from_one_to_three:
-    (shortest_path another_sample_graph 1 3) = [1;2;3].
+      (shortest_path another_sample_graph 1 3) = [1;2;3].
 Proof.
-    auto.
+      auto.
 Qed.
 
 Lemma shortest_path_from_one_to_seven:
-    (shortest_path another_sample_graph 1 7) = [1;5;7].
+      (shortest_path another_sample_graph 1 7) = [1;5;7].
 Proof.
-    auto.
+      auto.
 Qed.
 
 Lemma shortest_path_from_one_to_eight:
-    (shortest_path another_sample_graph 1 8) = [1;5;7;8].
+      (shortest_path another_sample_graph 1 8) = [1;5;7;8].
 Proof.
-    auto.
+      auto.
 Qed.
+
+(* 
+	Here we try to prove that the shortest path from a node to itself uses only one node
+*)
 
 Lemma shortest_path_from_five_to_one:
-    (shortest_path another_sample_graph 5 1) = [].
+      (shortest_path another_sample_graph 5 1) = [].
 Proof.
-    auto.
+      auto.
 Qed.
 
+Lemma a_greater_than_1_implies_a_star_a_greater_than_1:
+    forall (a: nat), a >= 1 -> (a*a) >= 1.
+Proof.
+    intros. assert (1 = 1*1) as Hx. auto. rewrite Hx. 
+    apply Nat.mul_le_mono. auto. auto.
+Qed.
 
+Lemma equality_of_decidable_nat:
+    forall (n: nat), (n =? n) = true.
+Proof.
+    intros. destruct (n =? n) eqn:Heq.
+    - reflexivity.
+    - rewrite Nat.eqb_neq in Heq.
+      exfalso. apply Heq.
+      reflexivity.
+Qed.
+
+Theorem shortest_path_helper_to_self_is_of_length_one:
+    forall g v fuel, fuel >= 1 -> (shortest_path_helper g [v] v [] fuel) = [v].
+Proof. 
+    intros. destruct fuel.
+    - inversion H.
+    - simpl. destruct (v =? v) eqn:Hx. auto. 
+    specialize (equality_of_decidable_nat v). intro. 
+    rewrite Hx in H0. inversion H0.
+Qed.
+
+Theorem shortest_path_to_self:
+    forall g v, (length g) >= 1 -> length(shortest_path g v v) = 1.
+Proof.
+    intros. simpl. unfold shortest_path. assert (length g * length g >= 1). 
+    apply a_greater_than_1_implies_a_star_a_greater_than_1. auto.
+    destruct (length g * length g) eqn:Hx.
+    - inversion H0.
+    - specialize (shortest_path_helper_to_self_is_of_length_one   g v (S n)). 
+    intro. assert (shortest_path_helper g [v] v [] (S n) = [v]).
+    apply H1. apply H0. rewrite H2. simpl. 
+    specialize (equality_of_decidable_nat v). intro. rewrite H3. auto.
+Qed.
+
+(* 
+	Identifying Bipartite Graphs
+	Below is a function that decides whether a graph is bipartite
+*)
+
+Fixpoint bipartite_helper (g : Graph) (visited stack left right : list Node) (fuel : nat) : (list Node * list Node * list Node) :=
+    match fuel with
+    | 0 => visited
+    | S fuel' =>
+          match stack with
+          | [] => (visited, left, right)
+          | vertex :: rem =>
+                if (existsb (Nat.eqb vertex) visited)
+                  then dfs_helper g visited rem fuel'
+                  else dfs_helper g ([vertex] ++ visited) ((get_children g vertex) ++ rem) fuel'
+          end
+    end.
+
+
+Fixpoint has_intersection (l1 l2 : list nat) : bool :=
+  match l1 with
+  | nil => false 
+  | x :: xs => if existsb (Nat.eqb x) l2 then true else has_intersection xs l2
+  end.
+
+Fixpoint is_bipartite_helper (g: Graph) (left: list Node) (right: list Node) : bool * list Node * list Node := 
+	match g with
+	| nil => (true, left, right)
+	| (v,e)::xg => if (existsb (Nat.eqb v) left) then
+		(
+			if (existsb (Nat.eqb v) right) then
+			(false, left, right)
+			else if (has_intersection (get_children g v) left) then
+			(false, left, right)
+			else (is_bipartite_helper xg ((get_children g v) ++ right) (v::left))
+		)
+		else (
+			if (has_intersection (get_children g v) right) then
+			(false, left, right)
+			else (is_bipartite_helper xg ((get_children g v) ++ left) (v::right))
+		)
+	end.
+
+Definition is_bipartite (g: Graph) : bool * list Node * list Node := 
+	(is_bipartite_helper g [] []).
+
+(* 
+	Again we begin by verifying the above works on some basic graphs
+	Consider the following graphs
+	1 --- 4
+	   /
+	2 --- 5
+	   /
+	3 --- 6
+	
+	7 --- 8
+	
+	9     
+*)
+
+Definition a_bipartite_graph := 
+	construct_dir_graph 4 [(1,4); (2,4)].
+
+Compute is_bipartite a_bipartite_graph.
+
+Lemma a_bipartite_graph_is_bipartite :
+	fst (fst (is_bipartite a_bipartite_graph)) = true.
+Proof.
+	unfold is_bipartite. unfold is_bipartite_helper.
+Qed.
 
 
 
@@ -697,12 +811,12 @@ Qed.
 
 
 Theorem dfs_implies_dfs_step_new: 
-    forall g start v fuel, 
-    In v (dfs_helper g [] [start] fuel) -> exists visited stack, DfsStepStar(g, [], [start])(g, v::visited, stack).
+      forall g start v fuel, 
+      In v (dfs_helper g [] [start] fuel) -> exists visited stack, DfsStepStar(g, [], [start])(g, v::visited, stack).
 Proof.
-    intros. induction fuel.
-    - destruct H.
-    - simpl in H. induction IHfuel. inversion H0.  
+      intros. induction fuel.
+      - destruct H.
+      - simpl in H. induction IHfuel. inversion H0.   
 Admitted.
 
 
